ImpE.v
@@ -676,7 +676,7 @@ Section Axioms.
   
   Axiom No_Pointers : forall (m: mem) l l', m l <> Vloc l'.
 
-  Definition meminit_wf d := forall l,
+  Definition meminit_wf minit d := forall l,
       match minit l with
       | Vlambda md c => forall Gm p Gp q rt,
                         Loc_Contxt l = Some (Typ (Tlambda Gm p md Gp) q, rt) ->
@@ -685,11 +685,12 @@ Section Axioms.
       | Vnat n => True
       end.
 
-  Axiom wf_minit : forall d, meminit_wf d.
+  Axiom wf_minit : forall d, meminit_wf minit d.
 
   Axiom Initial_State: forall d r' m',
       exists c md tr, cstep md d (c,reg_init,minit) (r',m') tr.
 
+  (* These next three axioms should follow from the statement of initial state above *)
   Axiom Reg_Exp_Lambda : forall (r : reg) d x md c G Gm Gp p q,
       r x = Vlambda md c /\ G x = Some (Typ (Tlambda Gm p md Gp) q)
       <-> exists md', exp_type md' G d (Elambda md c)
